code/experimental/rsa/Hacl.Test.RSA.fst
@@ -13,26 +13,26 @@ open Hacl.RSAPSS
 module Buffer = Spec.Lib.IntBuf
 
 val ctest:
-    x0:size_nat{x0 >= 6} ->
-    modBits:size_t -> n:lbytes (v (bits_to_text modBits)) ->
-    pkeyBits:size_t -> e:lbytes (v (bits_to_text pkeyBits)) ->
-    skeyBits:size_t -> d:lbytes (v (bits_to_text skeyBits)) ->
+    pow2_i:size_t ->
+    modBits:size_t -> n:lbytes (v (blocks modBits (size 8))) ->
+    pkeyBits:size_t -> e:lbytes (v (blocks pkeyBits (size 8))) ->
+    skeyBits:size_t -> d:lbytes (v (blocks skeyBits (size 8))) ->
     pTLen:size_t -> p:lbytes (v pTLen) ->
     qTLen:size_t -> q:lbytes (v qTLen) ->
     rBlindTLen:size_t -> rBlind:lbytes (v rBlindTLen) ->
     msgLen:size_t -> msg:lbytes (v msgLen) ->
     saltLen:size_t -> salt:lbytes (v saltLen) ->
-    sgnt_expected:lbytes (v (bits_to_text modBits)) -> Stack bool
+    sgnt_expected:lbytes (v (blocks modBits (size 8))) -> Stack bool
     (requires (fun h -> True))
     (ensures  (fun h0 r h1 -> True))
-let ctest x0 modBits n pkeyBits e skeyBits d pTLen p qTLen q rBlindTLen rBlind msgLen msg saltLen salt sgnt_expected =
-    let pow2_i = size (pow2 (x0 - 6)) in
-    let nLen = bits_to_bn modBits in
-    let eLen = bits_to_bn pkeyBits in
-    let dLen = bits_to_bn skeyBits in
-    let pLen = get_size_nat pTLen in
-    let qLen = get_size_nat qTLen in
-    let rBlindLen = get_size_nat rBlindTLen in
+let ctest pow2_i modBits n pkeyBits e skeyBits d pTLen p qTLen q rBlindTLen rBlind msgLen msg saltLen salt sgnt_expected =
+    //let pow2_i = size (pow2 (x0 - 6)) in
+    let nLen = blocks modBits (size 64) in
+    let eLen = blocks pkeyBits (size 64) in
+    let dLen = blocks skeyBits (size 64) in
+    let pLen = blocks pTLen (size 8) in
+    let qLen = blocks qTLen (size 8) in
+    let rBlindLen = blocks rBlindTLen (size 8) in
 
     let pkeyLen:size_t = add #SIZE nLen eLen in
     let skeyLen:size_t = add #SIZE (add #SIZE (add #SIZE pkeyLen dLen) pLen) qLen in
@@ -44,9 +44,9 @@ let ctest x0 modBits n pkeyBits e skeyBits d pTLen p qTLen q rBlindTLen rBlind m
     let pNat = Buffer.sub skey (add #SIZE pkeyLen dLen) pLen in
     let qNat = Buffer.sub skey (add #SIZE (add #SIZE pkeyLen dLen) pLen) qLen in
 
-    text_to_nat (bits_to_text modBits) n nNat;
-    text_to_nat (bits_to_text pkeyBits) e eNat;
-    text_to_nat (bits_to_text skeyBits) d dNat;
+    text_to_nat (blocks modBits (size 8)) n nNat;
+    text_to_nat (blocks pkeyBits (size 8)) e eNat;
+    text_to_nat (blocks skeyBits (size 8)) d dNat;
     text_to_nat pTLen p pNat;
     text_to_nat qTLen q qNat;
     
@@ -56,7 +56,7 @@ let ctest x0 modBits n pkeyBits e skeyBits d pTLen p qTLen q rBlindTLen rBlind m
     text_to_nat rBlindTLen rBlind rBlindNat;
     let rBlind0 = rBlindNat.(size 0) in
     
-    let nTLen = bits_to_text modBits in
+    let nTLen = blocks modBits (size 8) in
     let sgnt:lbytes (v nTLen) = Buffer.create nTLen (u8 0) in
     rsa_pss_sign #(v saltLen) #(v msgLen) #(v nLen) pow2_i modBits pkeyBits skeyBits pLen qLen skey rBlind0 saltLen salt msgLen msg sgnt;
     let check_sgnt = eq_b nTLen sgnt sgnt_expected in
@@ -68,7 +68,7 @@ val test1: unit -> Stack bool
     (ensures  (fun h0 r h1 -> True))
 let test1() =
     let modBits = size 1024 in
-    let nLen = bits_to_text modBits in
+    let nLen = blocks modBits (size 8) in
     let n : lbytes (v nLen) = Buffer.createL [
 	u8 0xa5; u8 0x6e; u8 0x4a; u8 0x0e; u8 0x70; u8 0x10; u8 0x17; u8 0x58; u8 0x9a; u8 0x51; u8 0x87; u8 0xdc; u8 0x7e; u8 0xa8; u8 0x41; u8 0xd1;
 	u8 0x56; u8 0xf2; u8 0xec; u8 0x0e; u8 0x36; u8 0xad; u8 0x52; u8 0xa4; u8 0x4d; u8 0xfe; u8 0xb1; u8 0xe6; u8 0x1f; u8 0x7a; u8 0xd9; u8 0x91;
@@ -79,10 +79,10 @@ let test1() =
 	u8 0x05; u8 0xac; u8 0xc2; u8 0xd3; u8 0xf0; u8 0xcb; u8 0x35; u8 0xf2; u8 0x92; u8 0x80; u8 0xe1; u8 0x38; u8 0x6b; u8 0x6f; u8 0x64; u8 0xc4;
 	u8 0xef; u8 0x22; u8 0xe1; u8 0xe1; u8 0xf2; u8 0x0d; u8 0x0c; u8 0xe8; u8 0xcf; u8 0xfb; u8 0x22; u8 0x49; u8 0xbd; u8 0x9a; u8 0x21; u8 0x37] in
     let pkeyBits = size 24 in
-    let eLen = bits_to_text pkeyBits in
+    let eLen = blocks pkeyBits (size 8) in
     let e : lbytes (v eLen) = Buffer.createL [u8 0x01; u8 0x00; u8 0x01] in
     let skeyBits = size 1024 in
-    let dLen = bits_to_text skeyBits in
+    let dLen = blocks skeyBits (size 8) in
     let d : lbytes (v dLen) = Buffer.createL [
         u8 0x33; u8 0xa5; u8 0x04; u8 0x2a; u8 0x90; u8 0xb2; u8 0x7d; u8 0x4f; u8 0x54; u8 0x51; u8 0xca; u8 0x9b; u8 0xbb; u8 0xd0; u8 0xb4; u8 0x47;
 	u8 0x71; u8 0xa1; u8 0x01; u8 0xaf; u8 0x88; u8 0x43; u8 0x40; u8 0xae; u8 0xf9; u8 0x88; u8 0x5f; u8 0x2a; u8 0x4b; u8 0xbe; u8 0x92; u8 0xe8;
@@ -125,7 +125,7 @@ let test1() =
         u8 0x1c; u8 0x8c; u8 0x9e; u8 0x3e; u8 0x99; u8 0x41; u8 0x54; u8 0xa9; u8 0x33; u8 0x95; u8 0xa5; u8 0x11; u8 0xb4; u8 0xa1; u8 0x72; u8 0xf6;
         u8 0x64; u8 0x4f; u8 0x37; u8 0xf6; u8 0x80; u8 0x7b; u8 0x86; u8 0x71; u8 0x6f; u8 0xc9; u8 0x07; u8 0xe1; u8 0xd0; u8 0xfc; u8 0x75; u8 0xbd;
         u8 0xa7; u8 0x7e; u8 0x41; u8 0x1b; u8 0xfc; u8 0x60; u8 0xfd; u8 0x2e; u8 0xd9; u8 0x27; u8 0x8e; u8 0x92; u8 0x1a; u8 0x33; u8 0x02; u8 0x1f] in
-    let res = ctest 10 modBits n pkeyBits e skeyBits d pLen p qLen q rBlindLen rBlind msgLen msg saltLen salt sgnt_expected in
+    let res = ctest (size 16) modBits n pkeyBits e skeyBits d pLen p qLen q rBlindLen rBlind msgLen msg saltLen salt sgnt_expected in
     res
 
 val test2: unit -> Stack bool
@@ -133,7 +133,7 @@ val test2: unit -> Stack bool
     (ensures  (fun h0 r h1 -> True))
 let test2() =
     let modBits = size 1025 in
-    let nLen = bits_to_text modBits in
+    let nLen = blocks modBits (size 8) in
     let n : lbytes (v nLen) = Buffer.createL [
         u8 0x01; u8 0xd4; u8 0x0c; u8 0x1b; u8 0xcf; u8 0x97; u8 0xa6; u8 0x8a; u8 0xe7; u8 0xcd; u8 0xbd; u8 0x8a; u8 0x7b; u8 0xf3; u8 0xe3; u8 0x4f;
         u8 0xa1; u8 0x9d; u8 0xcc; u8 0xa4; u8 0xef; u8 0x75; u8 0xa4; u8 0x74; u8 0x54; u8 0x37; u8 0x5f; u8 0x94; u8 0x51; u8 0x4d; u8 0x88; u8 0xfe;
@@ -145,10 +145,10 @@ let test2() =
         u8 0xfb; u8 0x42; u8 0xf8; u8 0xfc; u8 0x3d; u8 0x17; u8 0x6a; u8 0x01; u8 0x7e; u8 0xdc; u8 0x61; u8 0xfd; u8 0x32; u8 0x6c; u8 0x4b; u8 0x33;
         u8 0xc9 ] in
     let pkeyBits = size 24 in
-    let eLen = bits_to_text pkeyBits in
+    let eLen = blocks pkeyBits (size 8) in
     let e : lbytes (v eLen) = Buffer.createL [u8 0x01; u8 0x00; u8 0x01] in
     let skeyBits = size 1024  in
-    let dLen = bits_to_text skeyBits in
+    let dLen = blocks skeyBits (size 8) in
     let d : lbytes (v dLen) = Buffer.createL [
         u8 0x02; u8 0x7d; u8 0x14; u8 0x7e; u8 0x46; u8 0x73; u8 0x05; u8 0x73; u8 0x77; u8 0xfd; u8 0x1e; u8 0xa2; u8 0x01; u8 0x56; u8 0x57; u8 0x72;
         u8 0x17; u8 0x6a; u8 0x7d; u8 0xc3; u8 0x83; u8 0x58; u8 0xd3; u8 0x76; u8 0x04; u8 0x56; u8 0x85; u8 0xa2; u8 0xe7; u8 0x87; u8 0xc2; u8 0x3c;
@@ -205,7 +205,7 @@ let test2() =
         u8 0x92; u8 0x72; u8 0xc5; u8 0xd7; u8 0x73; u8 0x36; u8 0x8a; u8 0xbc; u8 0x06; u8 0x84; u8 0xd6; u8 0xbc; u8 0xc1; u8 0x9d; u8 0x30; u8 0x27;
         u8 0x73; u8 0x24; u8 0x54; u8 0x3e; u8 0xcd; u8 0xaf; u8 0x56; u8 0xf7; u8 0x44; u8 0x6e; u8 0x20; u8 0x79; u8 0xb8; u8 0x9c; u8 0xc4; u8 0x8f;
         u8 0x2d ] in
-    let res = ctest 11 modBits n pkeyBits e skeyBits d pLen p qLen q rBlindLen rBlind msgLen msg saltLen salt sgnt_expected in
+    let res = ctest (size 32) modBits n pkeyBits e skeyBits d pLen p qLen q rBlindLen rBlind msgLen msg saltLen salt sgnt_expected in
     res
 
 val test3: unit -> Stack bool
@@ -213,7 +213,7 @@ val test3: unit -> Stack bool
     (ensures  (fun h0 r h1 -> True))
 let test3() =
     let modBits = size 1536 in
-    let nLen = bits_to_text modBits in
+    let nLen = blocks modBits (size 8) in
     let n :lbytes (v nLen) = Buffer.createL [
         u8 0xe6; u8 0xbd; u8 0x69; u8 0x2a; u8 0xc9; u8 0x66; u8 0x45; u8 0x79; u8 0x04; u8 0x03; u8 0xfd; u8 0xd0; u8 0xf5; u8 0xbe; u8 0xb8; u8 0xb9;
         u8 0xbf; u8 0x92; u8 0xed; u8 0x10; u8 0x00; u8 0x7f; u8 0xc3; u8 0x65; u8 0x04; u8 0x64; u8 0x19; u8 0xdd; u8 0x06; u8 0xc0; u8 0x5c; u8 0x5b;
@@ -228,10 +228,10 @@ let test3() =
         u8 0x73; u8 0x57; u8 0xe1; u8 0xd3; u8 0x0e; u8 0x46; u8 0x31; u8 0x39; u8 0x81; u8 0x5c; u8 0x6f; u8 0xd4; u8 0xfd; u8 0x5a; u8 0xc5; u8 0xb8;
         u8 0x17; u8 0x2a; u8 0x45; u8 0x23; u8 0x0e; u8 0xcb; u8 0x63; u8 0x18; u8 0xa0; u8 0x4f; u8 0x14; u8 0x55; u8 0xd8; u8 0x4e; u8 0x5a; u8 0x8b] in
     let pkeyBits = size 24 in
-    let eLen = bits_to_text pkeyBits in
+    let eLen = blocks pkeyBits (size 8) in
     let e : lbytes (v eLen) = Buffer.createL [u8 0x01; u8 0x00; u8 0x01] in
     let skeyBits = size 1536 in 
-    let dLen = bits_to_text skeyBits in
+    let dLen = blocks skeyBits (size 8) in
     let d : lbytes (v dLen) = Buffer.createL [
         u8 0x6a; u8 0x7f; u8 0xd8; u8 0x4f; u8 0xb8; u8 0x5f; u8 0xad; u8 0x07; u8 0x3b; u8 0x34; u8 0x40; u8 0x6d; u8 0xb7; u8 0x4f; u8 0x8d; u8 0x61;
         u8 0xa6; u8 0xab; u8 0xc1; u8 0x21; u8 0x96; u8 0xa9; u8 0x61; u8 0xdd; u8 0x79; u8 0x56; u8 0x5e; u8 0x9d; u8 0xa6; u8 0xe5; u8 0x18; u8 0x7b;
@@ -289,7 +289,7 @@ let test3() =
         u8 0xfe; u8 0x74; u8 0xe4; u8 0x12; u8 0x26; u8 0x84; u8 0x71; u8 0xc9; u8 0x51; u8 0x81; u8 0x62; u8 0x51; u8 0x6c; u8 0xd6; u8 0xf9; u8 0x66;
         u8 0x89; u8 0x2a; u8 0x74; u8 0x0e; u8 0x1b; u8 0x8a; u8 0x88; u8 0x76; u8 0x6a; u8 0x30; u8 0xfc; u8 0xe9; u8 0xb6; u8 0x0e; u8 0x03; u8 0x32;
         u8 0xd7; u8 0xa0; u8 0x1b; u8 0xa5; u8 0xfa; u8 0x13; u8 0x5f; u8 0xe7; u8 0xc4; u8 0x92; u8 0x72; u8 0xac; u8 0xbb; u8 0x1d; u8 0x30; u8 0xf1] in
-    let res = ctest 11 modBits n pkeyBits e skeyBits d pLen p qLen q rBlindLen rBlind msgLen msg saltLen salt sgnt_expected in
+    let res = ctest (size 32) modBits n pkeyBits e skeyBits d pLen p qLen q rBlindLen rBlind msgLen msg saltLen salt sgnt_expected in
     res
 
 val test4: unit -> Stack bool
@@ -297,7 +297,7 @@ val test4: unit -> Stack bool
     (ensures  (fun h0 r h1 -> True))
 let test4() =
     let modBits = size 2048 in
-    let nLen = bits_to_text modBits in
+    let nLen = blocks modBits (size 8) in
     let n : lbytes (v nLen) = Buffer.createL [
         u8 0xa5; u8 0xdd; u8 0x86; u8 0x7a; u8 0xc4; u8 0xcb; u8 0x02; u8 0xf9; u8 0x0b; u8 0x94; u8 0x57; u8 0xd4; u8 0x8c; u8 0x14; u8 0xa7; u8 0x70;
         u8 0xef; u8 0x99; u8 0x1c; u8 0x56; u8 0xc3; u8 0x9c; u8 0x0e; u8 0xc6; u8 0x5f; u8 0xd1; u8 0x1a; u8 0xfa; u8 0x89; u8 0x37; u8 0xce; u8 0xa5;
@@ -316,10 +316,10 @@ let test4() =
         u8 0x1a; u8 0x73; u8 0x81; u8 0x98; u8 0xee; u8 0x27; u8 0xcf; u8 0x55; u8 0xa1; u8 0x3b; u8 0x75; u8 0x45; u8 0x39; u8 0x90; u8 0x65; u8 0x82;
         u8 0xec; u8 0x8b; u8 0x17; u8 0x4b; u8 0xd5; u8 0x8d; u8 0x5d; u8 0x1f; u8 0x3d; u8 0x76; u8 0x7c; u8 0x61; u8 0x37; u8 0x21; u8 0xae; u8 0x05] in
     let pkeyBits = size 24 in
-    let eLen = bits_to_text pkeyBits in
+    let eLen = blocks pkeyBits (size 8) in
     let e : lbytes (v eLen) = Buffer.createL [u8 0x01; u8 0x00; u8 0x01] in
     let skeyBits = size 2048 in
-    let dLen = bits_to_text skeyBits in
+    let dLen = blocks skeyBits (size 8) in
     let d : lbytes (v dLen) = Buffer.createL [
         u8 0x2d; u8 0x2f; u8 0xf5; u8 0x67; u8 0xb3; u8 0xfe; u8 0x74; u8 0xe0; u8 0x61; u8 0x91; u8 0xb7; u8 0xfd; u8 0xed; u8 0x6d; u8 0xe1; u8 0x12;
         u8 0x29; u8 0x0c; u8 0x67; u8 0x06; u8 0x92; u8 0x43; u8 0x0d; u8 0x59; u8 0x69; u8 0x18; u8 0x40; u8 0x47; u8 0xda; u8 0x23; u8 0x4c; u8 0x96;
@@ -390,7 +390,7 @@ let test4() =
         u8 0x95; u8 0x25; u8 0x65; u8 0xb8; u8 0xa1; u8 0x9a; u8 0x8f; u8 0xc3; u8 0xf0; u8 0xee; u8 0x7d; u8 0x39; u8 0x1d; u8 0x9b; u8 0x8b; u8 0x3f;
         u8 0x98; u8 0xbe; u8 0xbb; u8 0x0d; u8 0x5d; u8 0x01; u8 0x0e; u8 0x32; u8 0xe0; u8 0xb8; u8 0x00; u8 0xe9; u8 0x65; u8 0x6f; u8 0x64; u8 0x08;
         u8 0x2b; u8 0xb1; u8 0xac; u8 0x95; u8 0xa2; u8 0x23; u8 0xf4; u8 0x31; u8 0xec; u8 0x40; u8 0x6a; u8 0x42; u8 0x95; u8 0x4b; u8 0x2d; u8 0x57] in
-    let res = ctest 11 modBits n pkeyBits e skeyBits d pLen p qLen q rBlindLen rBlind msgLen msg saltLen salt sgnt_expected in
+    let res = ctest (size 32) modBits n pkeyBits e skeyBits d pLen p qLen q rBlindLen rBlind msgLen msg saltLen salt sgnt_expected in
     res
 
 val main: unit -> Stack FStar.Int32.t
@@ -398,5 +398,5 @@ val main: unit -> Stack FStar.Int32.t
     (ensures  (fun h0 r h1 -> True))
 let main () =
     let test = test1() && test2() && test3() && test4() in
-    if test then C.String.print (C.String.of_literal "SUCCESS") else C.String.print (C.String.of_literal "Test failed");
+    if test then C.String.print (C.String.of_literal "SUCCESS\n") else C.String.print (C.String.of_literal "Test failed\n");
     1l
