code/experimental/rsa/Hacl.Impl.Lib.fst
@@ -17,19 +17,6 @@ val blocks: x:size_t{v x > 0} -> m:size_t{v m > 0} -> r:size_t{v r > 0 /\ v x <=
 [@ "substitute"]
 let blocks x m = add_mod #SIZE ((sub_mod #SIZE x (size 1)) /. m) (size 1)
 
-(* text_to_bn *)
-val get_size_nat: lenText:size_t{v lenText > 0} -> Tot (res:size_t{v res > 0})
-[@ "substitute"]
-let get_size_nat lenText = blocks lenText (size 8)
-
-val bits_to_bn: bits:size_t{v bits > 0} -> Tot (res:size_t{v res > 0})
-[@ "substitute"]
-let bits_to_bn bits = blocks bits (size 64)
-
-val bits_to_text: bits:size_t{v bits > 0} -> Tot (res:size_t{v res > 0})
-[@ "substitute"]
-let bits_to_text bits = blocks bits (size 8)
-
 val eq_u64: a:uint64 -> b:uint64 -> Tot bool
 [@ "substitute"]
 let eq_u64 a b = FStar.UInt64.(u64_to_UInt64 a =^ u64_to_UInt64 b)
@@ -48,77 +35,86 @@ let eq_u8 a b = FStar.UInt8.(u8_to_UInt8 a =^ u8_to_UInt8 b)
 
 (* check if input[ind] is equal to 1 *)
 val bn_is_bit_set:
-    #len:size_nat -> clen:size_t{v clen == len} ->
-    input:lbignum len ->
-    ind:size_t{v ind / 64 < len} -> Stack bool
-    (requires (fun h -> live h input))
-    (ensures  (fun h0 r h1 -> preserves_live h0 h1 /\ h0 == h1))
-    [@"c_inline"]
+  #len:size_nat -> clen:size_t{v clen == len} ->
+  input:lbignum len ->
+  ind:size_t{v ind / 64 < len} -> Stack bool
+  (requires (fun h -> live h input))
+  (ensures  (fun h0 r h1 -> preserves_live h0 h1 /\ h0 == h1))
+  [@"c_inline"]
 let bn_is_bit_set #len clen input ind =
-    let i = ind /. size 64 in
-    let j = ind %. size 64 in
-    let tmp = input.(i) in
-    let tmp = (shift_right #U64 tmp (size_to_uint32 j)) &. u64 1 in
-    eq_u64 tmp (u64 1)
+  let i = ind /. size 64 in
+  let j = ind %. size 64 in
+  let tmp = input.(i) in
+  let tmp = (shift_right #U64 tmp (size_to_uint32 j)) &. u64 1 in
+  eq_u64 tmp (u64 1)
 
 val bn_set_bit:
-    #len:size_nat -> clen:size_t{v clen == len} ->
-    input:lbignum len ->
-    ind:size_t{v ind / 64 < len} -> Stack unit
-    (requires (fun h -> live h input))
-    (ensures  (fun h0 r h1 -> preserves_live h0 h1 /\ modifies1 input h0 h1))
-    [@"c_inline"]
+  #len:size_nat -> clen:size_t{v clen == len} ->
+  input:lbignum len ->
+  ind:size_t{v ind / 64 < len} -> Stack unit
+  (requires (fun h -> live h input))
+  (ensures  (fun h0 r h1 -> preserves_live h0 h1 /\ modifies1 input h0 h1))
+  [@"c_inline"]
 let bn_set_bit #len clen input ind =
-    let i = ind /. size 64 in
-    let j = ind %. size 64 in
-    let tmp = input.(i) in
-    input.(i) <- (tmp |. (shift_left #U64 (u64 1) (size_to_uint32 j)))
+  let i = ind /. size 64 in
+  let j = ind %. size 64 in
+  let tmp = input.(i) in
+  input.(i) <- (tmp |. (shift_left #U64 (u64 1) (size_to_uint32 j)))
 
 val bval:
-    #bLen:size_nat -> cbLen:size_t{v cbLen == bLen} ->
-    b:lbignum bLen -> i:size_t -> Stack uint64
-    (requires (fun h -> live h b))
-    (ensures (fun h0 _ h1 -> preserves_live h0 h1 /\ h0 == h1))
-    [@"c_inline"]
+  #bLen:size_nat -> cbLen:size_t{v cbLen == bLen} ->
+  b:lbignum bLen -> i:size_t -> Stack uint64
+  (requires (fun h -> live h b))
+  (ensures (fun h0 _ h1 -> preserves_live h0 h1 /\ h0 == h1))
+  [@"c_inline"]
 let bval #bLen cbLen b i =
-    if (i <. cbLen) then b.(i) else u64 0
+  if (i <. cbLen) then b.(i) else u64 0
 
 (* temporal functions *)
 val fill:
-    #len:size_nat -> clen:size_t{v clen == len} ->
-    b:lbignum len -> z:uint64 -> Stack unit
-    (requires (fun h -> live h b))
-    (ensures (fun h0 r h1 -> preserves_live h0 h1 /\ modifies1 b h0 h1))
-    [@"c_inline"]
+  #len:size_nat -> clen:size_t{v clen == len} ->
+  b:lbignum len -> z:uint64 -> Stack unit
+  (requires (fun h -> live h b))
+  (ensures (fun h0 r h1 -> preserves_live h0 h1 /\ modifies1 b h0 h1))
+  [@"c_inline"]
 let fill #len clen b z =
-    alloc #uint64 #unit #len clen z [] [BufItem b]
-    (fun h0 _ h1 -> True)
-    (fun tmp ->
-       copy clen tmp b
-    )
+  alloc #uint64 #unit #len clen z [] [BufItem b]
+  (fun h0 _ h1 -> True)
+  (fun tmp ->
+    copy clen tmp b
+  )
 
 val mul_wide: a:uint64 -> b:uint64 -> Tot uint128
 [@ "substitute"]
 let mul_wide a b = u128_from_UInt128 (FStar.UInt128.mul_wide (u64_to_UInt64 a) (u64_to_UInt64 b))
 
 val eq_b_:
-    #len:size_nat -> clen:size_t{v clen == len} ->
-    b1:lbytes len -> b2:lbytes len ->
-    i:size_t{v i <= len} -> Stack bool
-    (requires (fun h -> live h b1 /\ live h b2 /\ disjoint b1 b2))
-    (ensures (fun h0 _ h1 -> preserves_live h0 h1 /\ h0 == h1))
-    [@"c_inline"]
-let rec eq_b_ #len clen b1 b2 i =
-    if (i <. clen) then begin
-       if (eq_u8 b1.(i) b2.(i))
-       then eq_b_ #len clen b1 b2 (add #SIZE i (size 1))
-       else false end 
-    else true
+  #len:size_nat -> clen:size_t{v clen == len} ->
+  b1:lbytes len -> b2:lbytes len ->
+  res:lbuffer bool 1 -> Stack unit
+  (requires (fun h -> live h b1 /\ live h b2 /\ live h res))
+  (ensures (fun h0 _ h1 -> preserves_live h0 h1 /\ modifies1 res h0 h1))
+  [@ "substitute"]
+let eq_b_ #len clen b1 b2 res =
+  iteri_simple #bool #1 clen
+  (fun i res ->
+    let h = FStar.HyperStack.ST.get() in
+    assume (live h b1 /\ live h b2);
+    let a1 = res.(size 0) in
+    let a2 = eq_u8 b1.(i) b2.(i) in
+    res.(size 0) <- a1 && a2
+  ) res
 
 val eq_b:
-    #len:size_nat -> clen:size_t{v clen == len} ->
-    b1:lbytes len -> b2:lbytes len -> Stack bool
-    (requires (fun h -> live h b1 /\ live h b2 /\ disjoint b1 b2))
-    (ensures (fun h0 _ h1 -> preserves_live h0 h1 /\ h0 == h1))
-    [@"c_inline"]
-let eq_b #len clen b1 b2 = eq_b_ #len clen b1 b2 (size 0)
+  #len:size_nat -> clen:size_t{v clen == len} ->
+  b1:lbytes len -> b2:lbytes len -> Stack bool
+  (requires (fun h -> live h b1 /\ live h b2 /\ disjoint b1 b2))
+  (ensures (fun h0 _ h1 -> preserves_live h0 h1 /\ modifies0 h0 h1))
+  [@"c_inline"]
+let eq_b #len clen b1 b2 =
+  alloc #bool #bool #1 (size 1) (true) [BufItem b1; BufItem b2] []
+  (fun h0 _ h1 -> True)
+  (fun res ->
+    eq_b_ #len clen b1 b2 res;
+    res.(size 0)
+  )
